finish fundamental; helper lemmas left

SystemF.v
@@ -23,6 +23,8 @@ Inductive multi {X : Type} (R : relation X) : relation X :=
 						multi R y z ->
 						multi R x z.
 
+Hint Constructors multi : core.
+
 Module SystemF.
 
 (* ================================================================= *)
@@ -274,20 +276,23 @@ Hint Constructors step : core.
 Notation multistep := (multi step).
 Notation "e1 '-->*' e2" := (multistep e1 e2) (at level 40).
 
+Lemma step_trans : forall e1 e2 e3,
+	e1 -->* e2 ->
+	e2 -->* e3 ->
+	e1 -->* e3.
+Proof.
+Admitted.
 
 Definition normalises (e : tm) := exists v, value v /\ e -->* v.
 
 Example normalise_value : normalises (tm_abs (tm_var 0)).
 Proof.
 	exists (tm_abs (tm_var 0)). split; auto.
-	apply multi_refl.
 Qed.
 
 Example normalise_fun : normalises (tm_app (tm_abs (tm_var 0)) tm_unit).
 Proof.
-	exists <{()}>. split; auto.
-	eapply multi_step; auto.
-	apply multi_refl.
+	exists <{()}>. split; eauto.
 Qed.
 
 Example stuck : ~ normalises (<{fst () }>).
@@ -432,6 +437,13 @@ Fixpoint lr_val (xi : predCtxt) (t : ty) (v : tm) : Prop :=
 		(forall P, normalises_pred e (lr_val (P :: xi) T))
 	end.
 
+Fixpoint log_rel_seq (xi : predCtxt) (Gamma : varContext) (vs : list tm) : Prop :=
+	match Gamma with
+	| [] => vs = []
+	| t :: ts' =>
+		exists v vs', vs = v :: vs' /\ lr_val xi t v /\ log_rel_seq xi ts' vs'
+	end.
+
 (* ================================================================= *)
 (** ** Helper Lemmas *)
 
@@ -529,6 +541,21 @@ Proof.
 	apply log_rel_weaken_gen with (xi1 := []) (xi := [P]) (xi2 := xi); auto.
 Qed.
 
+Lemma log_rel_seq_weaken xi P Gamma vs :
+	log_rel_seq xi Gamma vs <-> log_rel_seq (P :: xi) (subst (ren (+1)) <$> Gamma) vs.
+Proof.
+	revert xi vs. induction Gamma; simpl; auto; intros; simpl.
+	split; intros.
+	- destruct H as [v [vs' [H1 [H2 H3]]]].
+		exists v, vs'. repeat (split; auto).
+		eapply log_rel_weaken in H2; eauto.
+		by apply IHGamma.
+	- destruct H as [v [vs' [H1 [H2 H3]]]].
+		exists v, vs'. repeat (split; auto).
+		eapply log_rel_weaken; eauto.
+		by apply IHGamma.
+Qed.
+
 Lemma log_rel_subst_gen xi' xi T T' v :
 	lr_val (xi' ++ xi) T.[upn (length xi') (T' .: ids)] v <-> lr_val (xi' ++ (lr_val xi T') :: xi) T v.
 Proof.
@@ -597,46 +624,139 @@ Proof.
 			symmetry in IHT. apply (IHT (P :: xi')). assumption.
 Qed.
 
+Lemma log_rel_subst xi T T' v :
+	lr_val xi T.[T'/] v <-> lr_val ((lr_val xi T') :: xi) T v.
+Proof.
+	apply log_rel_subst_gen with (xi' := []) (xi := xi); auto.
+Qed.
+
+Lemma norm_mono e P Q:
+	(forall v, P v -> Q v) ->
+	normalises_pred e P ->
+	normalises_pred e Q.
+Proof.
+	intros H1 H2. unfold normalises_pred in *.
+	destruct H2 as [v [? [? ?]]].
+	exists v. repeat (split; auto).
+Qed.
+
+Lemma norm_val v P:
+	value v ->
+	P v->
+	normalises_pred v P.
+Proof.
+	intros H1 H2. unfold normalises_pred in *.
+	exists v. repeat (split; auto).
+Qed.
 
 (* ################################################################# *)
 (** * Fundamental Theorem and Soundness *)
 
-Fixpoint log_rel_seq (xi : predCtxt) (Gamma : varContext) (vs : list tm) : Prop :=
-	match Gamma with
-	| [] => vs = []
-	| t :: ts' =>
-		exists v vs', vs = v :: vs' /\ lr_val xi t v /\ log_rel_seq xi ts' vs'
-	end.
+Fixpoint env_subst (vs : list tm) : var → tm :=
+  match vs with
+  | [] => ids
+  | v :: vs' => v .: env_subst vs'
+  end.
 
-(* Theorem fundamental_theorem : forall Gamma e vs T xi,
+Lemma subst_step_var Gamma x T vs xi:
+	Gamma !! x = Some T ->
+	log_rel_seq xi Gamma vs ->
+	normalises_pred (env_subst vs x) (lr_val xi T).
+Proof.
+Admitted.
+
+Lemma subst_step_pair e1 v1 e2 v2 vs:
+	e1.[env_subst vs] -->* v1 ->
+	value v1 ->
+	e2.[env_subst vs] -->* v2 ->
+	value v2 ->
+	tm_pair e1.[env_subst vs] e2.[env_subst vs] -->* <{(- v1, v2 -)}>.
+Proof.
+Admitted.
+
+Lemma subst_step_fst e v1 v2 vs:
+	e.[env_subst vs] -->* <{(- v1, v2 -)}> ->
+	value v1 ->
+	value v2 ->
+	tm_fst e.[env_subst vs] -->* v1.
+Proof.
+Admitted.
+
+Lemma subst_step_snd e v1 v2 vs:
+	e.[env_subst vs] -->* <{(- v1, v2 -)}> ->
+	value v1 ->
+	value v2 ->
+	tm_snd e.[env_subst vs] -->* v2.
+Proof.
+Admitted.
+
+Lemma subst_step_app e1 e e2 v vs v':
+	e1.[env_subst vs] -->* tm_abs e ->
+	e2.[env_subst vs] -->* v ->
+	value v ->
+	e.[v/] -->* v' ->
+	value v' ->
+	tm_app e1.[env_subst vs] e2.[env_subst vs] -->* v'.
+Proof.
+Admitted.
+
+Lemma subst_step_tapp e b v0 vs:
+	e.[env_subst vs] -->* tm_tyabs b ->
+	b -->* v0 ->
+	value v0 ->
+	tm_tyapp e.[env_subst vs] -->* v0.
+Proof.
+Admitted.
+
+Theorem fundamental_theorem : forall Gamma e vs T xi,
 	Gamma |- e : T ->
 	log_rel_seq xi Gamma vs ->
-	normalises_pred e.[vs/] (lr_val xi T). *)
-
-Theorem fundamental_theorem_weak : forall e T xi,
-	[] |- e : T ->
-	normalises_pred e (lr_val xi T).
+	normalises_pred e.[env_subst vs] (lr_val xi T).
 Proof.
-	intros e T xi H. revert xi. remember [] as Gamma eqn:HGamma.
-	induction H; intros xi; subst; simpl.
-	- exists <{()}>. split; auto. split; auto using multi_refl.
-	- inversion H.
-	- assert (IH1: normalises_pred e1 (lr_val xi T1)) by auto.
-	  assert (IH2: normalises_pred e2 (lr_val xi T2)) by auto.
-	  unfold normalises_pred in *.
-	  destruct IH1 as [v1 [Hv1 [Hv1' Hv1'']]].
-	  destruct IH2 as [v2 [Hv2 [Hv2' Hv2'']]].
+	intros Gamma e vs T xi H. revert vs xi.
+	induction H; intros vs xi Hlog; simpl.
+	- unfold normalises_pred. exists <{()}>. split; auto.
+	- eapply subst_step_var; eauto.
+	- destruct (IHhas_type1 vs xi Hlog) as [v1 [Hv1 [Hv1' Hv1'']]].
+	  destruct (IHhas_type2 vs xi Hlog) as [v2 [Hv2 [Hv2' Hv2'']]].
+	  unfold normalises_pred.
 	  exists <{(- v1, v2 -)}>; repeat (auto; split).
-	  { admit. }
-	  exists v1, v2. split; auto; split; auto.
-	- assert (IH: normalises_pred e (lr_val xi <{ (~T1 * T2 ~) }>)) by auto.
-	  unfold normalises_pred in *.
-	  destruct IH as [v [Hv [Hv' Hv'']]].
-	  inversion Hv'' as [v1 [v2 [Hv1v2 [Hv1 Hv2]]]].
-	  subst; inversion Hv; subst.
-	  exists v1. split; auto; split; auto.
-	  admit.
-Admitted.
+	  { eapply subst_step_pair; eauto. }
+	  exists v1, v2. repeat (split; auto).
+	- destruct (IHhas_type vs xi Hlog) as [v [Hv [Hv' Hv'']]].
+	  inversion Hv'' as [v1 [v2 [Hv_eq [Hv1 Hv2]]]]; subst.
+	  exists v1. inversion Hv; subst. repeat (split; auto).
+	  eapply subst_step_fst; eauto.
+	- destruct (IHhas_type vs xi Hlog) as [v [Hv [Hv' Hv'']]].
+	  inversion Hv'' as [v1 [v2 [Hv_eq [Hv1 Hv2]]]]; subst.
+	  exists v2. inversion Hv; subst. repeat (split; auto).
+	  eapply subst_step_snd; eauto.
+	- apply norm_val; auto.
+	  exists e.[up (env_subst vs)]; split; auto.
+	  intros v Hv.
+	  assert (Hsubst: e.[up (env_subst vs)].[v/] = e.[env_subst (v :: vs)]) by by asimpl.
+	  rewrite Hsubst. apply IHhas_type. simpl; eauto.
+	- destruct (IHhas_type1 vs xi Hlog) as [v1 [Hv1 [Hv1' Hv1'']]].
+	  destruct (IHhas_type2 vs xi Hlog) as [v2 [Hv2 [Hv2' Hv2'']]].
+	  inversion Hv1'' as [e [He He']].
+	  apply He' in Hv2''.
+	  unfold normalises_pred in Hv2''.
+	  destruct Hv2'' as [v' [Hv' [Hv'' Hv''']]]; subst.
+	  exists v'. repeat (split; auto). subst.
+	  eapply subst_step_app; eauto.
+	- apply norm_val; auto.
+	  exists e.[env_subst vs]. split; auto.
+	  intros P.
+	  apply IHhas_type. simpl.
+	  by apply log_rel_seq_weaken.
+	- destruct (IHhas_type vs xi Hlog) as [v [Hv [Hv' Hv'']]].
+	  inversion Hv'' as [b [Hb Hb']]; subst.
+	  destruct (Hb' (lr_val xi T')) as [v0 [Hv0' [Hv0'' Hv0''']]].
+	  apply norm_mono with (P := lr_val (lr_val xi T' :: xi) T).
+	  apply log_rel_subst.
+	  exists v0. repeat (split; auto).
+	  apply subst_step_tapp with (b := b); auto.
+Qed.
 
 Theorem normalisation: forall e T,
 	[] |- e : T ->
